Added second branch test, increased qi threshold in testing

test/core/DY.Test.Core.Trace.Modifies.fst
@@ -30,6 +30,8 @@ let broad_unmodified_proof (prin:principal) (tr_in:trace)
   = let (new_sid, tr_out) = broad_unmodified_test prin tr_in in
     assert(traceful_modifies (broad_unmodified_test prin) tr_in == singleton (prin, new_sid))
 
+/// This test, similar to the previous, validates the modifies analysis, particularly
+/// ensuring that the traceful option bind with *? works as well.
 let optional_unmodified_test (prin:principal)
   : traceful (option state_id)
   = let* new_rand = mk_rand NoUsage (DY.Core.Label.principal_label prin) 32 in
@@ -53,6 +55,8 @@ let optional_unmodified_proof (prin:principal) (tr_in:trace)
     | None -> assert(traceful_modifies (optional_unmodified_test prin) tr_in == empty)
     | Some new_sid -> assert(traceful_modifies (optional_unmodified_test prin) tr_in `subset` singleton (prin, new_sid))
 
+/// The following tests ensure that the automation works despite branching, first
+/// within a pure value, and then in the control flow.
 assume val test_branch : bool
 
 let branch_unmodified_test (prin:principal)
@@ -60,15 +64,16 @@ let branch_unmodified_test (prin:principal)
   = let* new_rand = mk_rand NoUsage (DY.Core.Label.principal_label prin) 32 in
     let* msg_ts = send_msg new_rand in
     trigger_event prin "test_event" (Literal (Seq.Base.empty));*
-//  Adding this next line back in causes the automation below to fail.
-//  Something to do with needing to search too deep?
-//    let* _ = recv_msg msg_ts in
+    let* _ = recv_msg msg_ts in
     let* new_sid1 = new_session_id prin in
     let* new_sid2 = new_session_id prin in
     let modify_sid = if test_branch then new_sid1 else new_sid2 in
     let* _ = set_state prin modify_sid new_rand in
     return (new_sid1, new_sid2)
 
+/// Without this option, the proof automation gets stuck working through
+/// "extraneous" steps.
+#push-options "--z3cliopt 'smt.qi.eager_threshold=100'"
 let branch_unmodified_proof (prin:principal) (tr_in:trace)
   : Lemma
     (let ((new_sid1, new_sid2), tr_out) = branch_unmodified_test prin tr_in in
@@ -81,3 +86,34 @@ let branch_unmodified_proof (prin:principal) (tr_in:trace)
   = let ((new_sid1, new_sid2), tr_out) = branch_unmodified_test prin tr_in in
     assert(traceful_modifies (branch_unmodified_test prin) tr_in `subset` (as_set [(prin, new_sid1); (prin, new_sid2)]));
     ()
+#pop-options
+
+let branch_unmodified_test_2 (prin:principal)
+  : traceful (state_id & state_id)
+  = let* new_rand = mk_rand NoUsage (DY.Core.Label.principal_label prin) 32 in
+    let* msg_ts = send_msg new_rand in
+    trigger_event prin "test_event" (Literal (Seq.Base.empty));*
+    let* _ = recv_msg msg_ts in
+    let* new_sid1 = new_session_id prin in
+    let* new_sid2 = new_session_id prin in
+    if test_branch
+    then (
+      let* _ = set_state prin new_sid1 new_rand in
+      return (new_sid1, new_sid2)
+    )
+    else
+    return (new_sid1, new_sid2)
+
+#push-options "--z3cliopt 'smt.qi.eager_threshold=100'"
+let branch_unmodified_proof_2 (prin:principal) (tr_in:trace)
+  : Lemma
+    (let ((new_sid1, new_sid2), tr_out) = branch_unmodified_test_2 prin tr_in in
+     forall (sid:state_id). (
+       sid == new_sid1 \/
+       get_state_aux prin sid tr_in == get_state_aux prin sid tr_out
+     )
+    )
+  = let ((new_sid1, new_sid2), tr_out) = branch_unmodified_test_2 prin tr_in in
+    assert(traceful_modifies (branch_unmodified_test_2 prin) tr_in `subset` (singleton (prin, new_sid1)));
+    ()
+ #pop-options
